# Proposed delta to sdmx.ttl to support metadata sets and definitions
# As a side effect of the requirements for metadata it provides a 
# proposed basis for resolving issue 30.

@prefix rdf:            <http://www.w3.org/1999/02/22-rdf-syntax-ns#> .
@prefix rdfs:           <http://www.w3.org/2000/01/rdf-schema#> .
@prefix owl:            <http://www.w3.org/2002/07/owl#> .
@prefix xsd:            <http://www.w3.org/2001/XMLSchema#> .
@prefix skos:           <http://www.w3.org/2004/02/skos/core#> .
@prefix foaf:           <http://xmlns.com/foaf/0.1/> .
@prefix scovo:          <http://purl.org/NET/scovo#> .
@prefix void:           <http://rdfs.org/ns/void#> .
@prefix sdmx:           <http://purl.org/linked-data/sdmx#> .
@prefix sdmx-concept:   <http://purl.org/linked-data/sdmx/2009/concept#> .
@prefix sdmx-dimension: <http://purl.org/linked-data/sdmx/2009/dimension#> .
@prefix sdmx-attribute: <http://purl.org/linked-data/sdmx/2009/attribute#> .
@prefix sdmx-measure:   <http://purl.org/linked-data/sdmx/2009/measure#> .
@prefix dcterms:        <http://dublincore.org/documents/dcmi-terms/>.

# --- Properties for Metadata Sets and Definitions  --------------------------

sdmx:MetadataStructureDefinition a rdfs:Class, owl:Class;
    rdfs:label "Metadata structure definition"@en;
    rdfs:comment "Defines the structure of a MetadataSet"@en;
    rdfs:subClassOf sdmx:Structure;
    .

sdmx:MetadataReportStructure a rdfs:Class, owl:Class;
    rdfs:label "Metadata report structure"@en;
    rdfs:comment "Defines the structure of a single report within an MSD"@en;
	.
	
sdmx:metadataReportStructure a rdf:Property, owl:ObjectProperty;
    rdfs:label "metadata report structure"@en;
    rdfs:comment """designates a single report structure within an overall metadata structure definition"""@en;
    rdfs:domain sdmx:MetadataStructureDefinition;
    rdfs:range  sdmx:MetadataReportStructure ;
	.
	
sdmx:MetadataProperty a rdfs:Class, owl:Class;
    rdfs:label "Metadata property"@en;
    rdfs:comment """Class of properties used to provide metadata values in metadata reports (sdmx:MetadataSet)"""@en;
    rdfs:subClassOf sdmx:ComponentProperty;
    owl:disjointWith sdmx:MeasureProperty;
    owl:disjointWith sdmx:AttributeProperty;
    owl:disjointWith sdmx:DimensionProperty;
    .

sdmx:childComponents a rdf:Property, owl:ObjectProperty;
    rdfs:label "child components"@en;
    rdfs:comment """Used primarily in sdmx:MetadataStructureDefinitions to indicate a grouping of the metadata properties used for presentational purposes. The sub components should still be listed as sdmx:components of the structure but in the sdmx:componentOrder the group is represented by a single sdmx:ComponentSpecification which in turn lists the child components by means of this property"""@en;
    rdfs:domain sdmx:ComponentSpecification;
    rdfs:range  rdf:List;
    .

sdmx:MetadataSet a rdfs:Class, owl:Class;
     rdfs:label "Metadata set"@en;
     rdfs:comment """A collection of metadata resports"""@en;
     .

sdmx:metadata a rdf:Property, owl:ObjectProperty;
    rdfs:label "metadata"@en;
    rdfs:comment """Links an entity (from Observation up to DataFlow) to a corresponding metadata record."""@en;
    rdfs:range sdmx:MetadataSet;
    .

sdmx:MetadataReport a rdfs:Class, owl:Class;
     rdfs:label "Metadata report"@en;
     rdfs:comment """A metadata report (within an overall Metadata set) containing metadata via attached MetadataProperties"""@en;
     .

sdmx:metadataReport a rdf:Property, owl:ObjectProperty;
    rdfs:label "metadata report"@en;
    rdfs:comment """Links a Metadata set to one or more component reports"""@en;
    rdfs:domain sdmx:MetadataSet;
    rdfs:domain sdmx:MetadataReport;
    .
    
sdmx:reportStructure a rdf:Property, owl:ObjectProperty;
    rdfs:label "report structure"@en;
    rdfs:comment """Links an individual metadata report to the report structure it corresponds to"""@en;
    rdfs:domain sdmx:MetadataReport ;
    rdfs:range  sdmx:MetadataReportStructure ;
    .
    
sdmx:effectiveDate a rdf:Property, owl:DatatypeProperty;
    rdfs:label "effective date"@en;
    rdfs:comment """The date on which all the effectiveDate metadata in the metadata set is effective."""@en;
    rdfs:subPropertyOf dcterms:date;
    rdfs:range xsd:dateTime;
    .

sdmx:MetadataFlow a rdfs:Class, owl:Class;
    rdfs:label "Metadata flow"@en;
    rdfs:comment """A flow of Metadata sets"""@en;
    rdfs:subClassOf sdmx:Structured, sdmx:Flow;
    .

sdmx:metadataFlow a rdf:Property, owl:ObjectProperty;
    rdfs:label "metadata flow"@en;
    rdfs:comment """gives the metadata flow associated with a metadata set"""@en;
    rdfs:domain sdmx:MetadataSet;
    rdfs:range  sdmx:MetadataFlow;
    .

# --- Structure pattern  --------------------------

sdmx:Structure a rdfs:Class, owl:Class;
    rdfs:label "Structure"@en;
    rdfs:comment "Abstract class for defining the structure (ComponentProperties) that can be used in some data or metadata set"@en;
    .

sdmx:DataStructureDefinition rdfs:subClassOf sdmx:Structure .
sdmx:MetadataStructureDefinition rdfs:subClassOf sdmx:Structure .

sdmx:Structured a rdfs:Class, owl:Class;
    rdfs:label "Structured"@en;
    rdfs:comment """Abstract class for things whose Structure can be defined by an sdmx:Structure declaration, alternative name: StructureUsage"""@en;
    .

sdmx:DataSet rdfs:subClassOf sdmx:Structured .
sdmx:DataFlow rdfs:subClassOf sdmx:Structured .

sdmx:structure a rdf:Property, owl:ObjectProperty;
    rdfs:label "structure"@en;
    rdfs:domain sdmx:Structured;
    rdfs:range sdmx:Structure;
    .
    
sdmx:component a rdf:Property, owl:ObjectProperty;
    rdfs:label "component"@en;
    rdfs:domain sdmx:Structure;
    rdfs:range sdmx:ComponentProperty;
    .

sdmx:componentOrder a rdf:Property, owl:ObjectProperty;
    rdfs:label "component order"@en;
    rdfs:domain sdmx:Structure;
    rdfs:range rdf:List;
    rdfs:comment """Optional specification of the order in which dimensions (and optionally other components) should be used. Value is an rdf:List of sdmx:ComponentProperties or sdmx:ComponentSpecifications"""@en;
    .

# --- Flow pattern --------------------------

sdmx:Flow a rdfs:Class, owl:Class;
    rdfs:label "Flow"@en;
    rdfs:comment """Abstract information flow, can be either data or metadata"""@en;
    rdfs:subClassOf sdmx:Structured;
    .

sdmx:DataFlow     rdfs:subClassOf  sdmx:Flow .
sdmx:MetadataFlow rdfs:subClassOf  sdmx:Flow .

sdmx:controllingAgreement a rdf:Property, owl:ObjectProperty;
    rdfs:label "controlling agreement"@en;
    rdfs:domain sdmx:Flow;
    rdfs:range sdmx:ProvisionAgreement;
    .

# --- Extended structure entries --------------------------

sdmx:ComponentSpecification a rdfs:Class, owl:Class ;
    rdfs:label "Component specification"@en;
    rdfs:comment """Used to define properties of a component (attribute, dimension etc) which are specific to its usage in a DSD or MSD. This is used by including instances of sdmx:ComponentSpecification in place of the sdmx:ComponentProperty in an sdmx:componentOrder list"""@en;
    .

sdmx:specifiedComponent a rdf:Property, owl:ObjectProperty;
    rdfs:label "specified component"@en;
    rdfs:comment """Links a component specification to the component property that is being qualified"""@en;
    rdfs:domain sdmx:ComponentSpecification;
    rdfs:range  sdmx:ComponentProperty;
    .

sdmx:commponentRequired a rdf:Property, owl:DatatypeProperty;
    rdfs:label "component required"@en;
    rdfs:comment """Indicates whether a component property is required (true) or optional (false) in the context of a DSD or MSD"""@en;
    rdfs:domain sdmx:ComponentSpecifition;
    rdfs:range  xsd:boolean;
    .

# --- @@  --------------------------

